compiler/backend/proofs/stack_to_labProofScript.sml
@@ -762,6 +762,7 @@ Proof
   imp_res_tac state_rel_read_reg_FLOOKUP_regs >> rfs[] >> rw[] >>
   imp_res_tac state_rel_read_fp_reg_FLOOKUP_fp_regs >> rfs[] >> rw[] >>
   imp_res_tac word_sh_word_shift >>
+  simp[w2n_lt] >>
   full_simp_tac(srw_ss())[wordLangTheory.word_op_def] >> srw_tac[][] >>
   imp_res_tac state_rel_read_reg_FLOOKUP_regs >> rfs[] >> rw[] >>
   TRY ( full_simp_tac(srw_ss())[binop_upd_def] >> match_mp_tac set_var_upd_reg >> full_simp_tac(srw_ss())[] >> NO_TAC) >>
